Loda/PropSemantics.lean
@@ -20,27 +20,4 @@ def tyenv2prop (σ : Env.ValEnv) (δ : Env.CircuitEnv) (ctr : ℕ) (Γ: Env.TyEn
   | Ast.Ty.refin _ e => expr2prop σ δ ctr e
   | _ => True
 
-/-- Given a circuit `c`, produce the Prop that says
-1. for any choice of inputs of the correct field type,
-2. evaluating `c.body` yields a value `v`,
-3. and `v` satisfies the refinement predicate in `c.output`. -/
-def circuit2prop (p : ℕ) (δ : Env.CircuitEnv) (c : Circuit.Circuit) : Prop :=
-  ∀ (xs : List (ZMod p)),
-    -- require that the argument list `xs` matches `c.inputs` in length
-    xs.length = c.inputs.length →
-  let σ : Env.ValEnv :=
-    (c.inputs.zip xs).foldl (fun σ (xy : (String × Ast.Ty) × ZMod p) =>
-      let ((name, _), x) := xy; Env.setVal σ name (Ast.Value.vF p x)) (fun _ => Ast.Value.vStar)
-  let Γ : Env.TyEnv :=
-    (c.inputs.zip xs).foldl (fun Γ (xy : (String × Ast.Ty) × ZMod p) =>
-      let ((name, τ), _) := xy; Env.setTy Γ name τ) (fun _ => Ast.Ty.unit)
-  ∀ p ∈ (List.zip c.inputs xs), (tyenv2prop σ δ 1000 Γ p.fst.fst) →
-  match Eval.eval σ δ 1000 c.body with
-  | some _ =>
-    -- extract the refinement predicate φ from `c.output`
-    match c.output with
-    | (n, Ast.Ty.refin _ φ) => expr2prop σ δ 1000 φ
-    | _            => True
-  | none   => False
-
 end PropSemantics
